
\documentclass{scrreprt}

\usepackage{script_preset}

\begin{document}

\section{Convex functions}

Let $I \subset \mathbb{R}$.

\begin{definition}
  A function $\varphi: I \to \mathbb{R}$ is called convex, if
  \[
  \varphi (\lambda x + (1-\lambda)y) \leq \lambda \varphi(x) + (1-\lambda) \varphi(y).
  \]
\end{definition}

\begin{proposition}
Let $x < y \in \mathbb{R}$. The set $\{\lambda x + (1-\lambda)y \mid \lambda \in [0,1]\}$ is just the interval $[x,y]$. 
\end{proposition}

\begin{proof}
  ``$\subseteq$'': Show that $\lambda x + (1-\lambda)y \in [x,y]$. It is
  \[
  \lambda x + (1-\lambda)y \leq \lambda y + (1-\lambda)y = y
  \] 
  and
  \[
  \lambda x + (1-\lambda)y \geq \lambda x + (1-\lambda) x = x,
  \]
  thus $\lambda x + (1-\lambda)y \in [x,y]$.
  
  ``$\supseteq$'': Show that every $z \in [x,y]$ has a representation $z=\lambda x + (1-\lambda)y$. Assume $z \in (x,y)$ otherwise $\lambda=0$ or $\lambda=1$.

  Set $\lambda=\frac{z-y}{x-y} < 0$. Then
  \[
  \frac{z-y}{x-y} x + (1- \frac{z-y}{x-y}) y = \frac{xz-yx+yx-y^2-zy+y^2}{x-y} = z
  \]
  as desired.
  
\end{proof}



\end{document}
