\section{Convex functions}

\begin{definition}
  A function $\varphi: C \to \mathbb{R}$, defined on a convex subset $C$ of $\mathbb{R}$, is called convex, if for all $x,y \in C$ and $\lambda \in [0,1]$
  \[
  \varphi (\lambda x + (1-\lambda)y) \leq \lambda \varphi(x) + (1-\lambda) \varphi(y).
  \]
\end{definition}

\begin{proposition}
Let $x < y \in \mathbb{R}$. The set $\{\lambda x + (1-\lambda)y \mid \lambda \in [0,1]\}$ is just the interval $[x,y]$. 
\end{proposition}

\begin{proof}
  ``$\subseteq$'': Show that $\lambda x + (1-\lambda)y \in [x,y]$. It is
  \[
  \lambda x + (1-\lambda)y \leq \lambda y + (1-\lambda)y = y
  \] 
  and
  \[
  \lambda x + (1-\lambda)y \geq \lambda x + (1-\lambda) x = x,
  \]
  thus $\lambda x + (1-\lambda)y \in [x,y]$.
  
  ``$\supseteq$'': Show that every $z \in [x,y]$ has a representation $z=\lambda x + (1-\lambda)y$. Assume $z \in (x,y)$ otherwise $\lambda=0$ or $\lambda=1$.

  Set $\lambda=\frac{z-y}{x-y} < 0$. Then
  \[
  \frac{z-y}{x-y} x + (1- \frac{z-y}{x-y}) y = \frac{xz-yx+yx-y^2-zy+y^2}{x-y} = z
  \]
  as desired.
  
\end{proof}


\begin{definition}
  A function $\varphi: C \to \mathbb{R}$ is called strictly convex, if for all $x,y \in C$ with $x \neq y$ and $\lambda \in (0,1)$
  \[
  \varphi (\lambda x + (1-\lambda)y) < \lambda \varphi(x) + (1-\lambda) \varphi(y).
  \]
\end{definition}

\begin{proposition}\label{convex_eq}
  For a strictly convex function $\varphi: C \to \mathbb{R}$ the equality
  \[
  \varphi (\lambda x + (1-\lambda)y) = \lambda \varphi(x) + (1-\lambda) \varphi(y).
  \]
  holds if and only if x=y.
  
\end{proposition}

\begin{proof}
  Trivial. If $x=y$,
  \begin{align*}
    \varphi (\lambda x + (1-\lambda)y) &= \varphi (\lambda x + (1-\lambda)x) = \varphi(x)
    \\ &= \lambda \varphi(x) + (1-\lambda) \varphi(x) =\lambda \varphi(x) + (1-\lambda) \varphi(y).
  \end{align*}

  Conversely, assume $x \neq y$ and that the equality above holds. By the strict convexity of $\varphi$, we obtain
  \[
  \varphi (\lambda x + (1-\lambda)y) < \lambda \varphi(x) + (1-\lambda) \varphi(y) = \varphi(\lambda x + (1-\lambda)y),
  \]
  showing that $x=y$ must hold.
\end{proof}
